examples/Imp2Vir/Imp2Cvir.v
@@ -23,8 +23,9 @@ Open Scope Z_scope.
 
 Section Imp2Cvir.
 
+
   Fixpoint compile (next_reg : int) (s : stmt) (env: StringMap.t int)
-  : option (int * (StringMap.t int) * cvir 1 1) :=
+    : option (int * (StringMap.t int) * cvir 1 1) :=
     match s with
     | Skip => Some(next_reg, env, block_cvir [])
     | Assign x e =>
@@ -80,7 +81,6 @@ compile next_reg s env = Some(next_reg', env', ir) -> cvir_WF ir.
       apply seq_cvir_WF.
       apply branch_cvir_WF.
       apply merge_cvir_WF with (ni1:= 1%nat) (no1:= 1%nat) (ir1:= c0) in Heqo2 ; assumption.
-      (* I don't understand why `apply merge_cvir_WF`` doesn't work *)
     - repeat break_match ; try discriminate.
       inversion Heqo.
       subst.
@@ -93,40 +93,42 @@ compile next_reg s env = Some(next_reg', env', ir) -> cvir_WF ir.
                                  (ir1:= c0) (ir2:= (block_cvir [])) ;
           [ assumption | apply block_cvir_WF ].
     - inversion Heqo. apply block_cvir_WF.
-Qed.
+  Qed.
 
-Definition compile_imp_cvir (ir : cvir 1 1) : program :=
-  let ir := seq_cvir ir (ret_cvir nil (texp_i32 10)) in (* hack to print the result of fact *)
-  let vt_seq := map Anon (map Z.of_nat (seq 2 (n_int ir))) in
-  let blocks := (blocks ir) (cons (Anon 1) (empty raw_id)) (empty raw_id) vt_seq in
-  let body := (entry_block, blocks) in
-  let decl := mk_declaration
-    (Name "main")
-    (TYPE_Function (TYPE_I 32) [TYPE_I 64 ; TYPE_Pointer (TYPE_Pointer (TYPE_I 8))])
-    (nil, nil) None None None None nil None None None
-  in
-  let def := mk_definition fnbody decl nil body in
-  TLE_Definition def.
+  Definition compile_imp_cvir (ir : cvir 1 1) : program :=
+    let ir := seq_cvir ir (ret_cvir nil (texp_i32 10)) in (* hack to print the result of fact *)
+    let vt_seq := map Anon (map Z.of_nat (seq 2 (n_int ir))) in
+    let blocks := (blocks ir) (cons (Anon 1) (empty raw_id)) (empty raw_id) vt_seq in
+    let body := (entry_block, blocks) in
+    let decl := mk_declaration
+      (Name "main")
+      (TYPE_Function (TYPE_I 32) [TYPE_I 64 ; TYPE_Pointer (TYPE_Pointer (TYPE_I 8))])
+      (nil, nil) None None None None nil None None None
+    in
+    let def := mk_definition fnbody decl nil body in
+    TLE_Definition def.
 
-Definition compile_program (s : stmt) (env : StringMap.t int) :
-  option program :=
-  '(_, _, ir) <- compile 0 s env;;
-  ret (compile_imp_cvir ir).
-
-
-
-Definition fact_ir := (compile_program (fact "a" "b" 5) (StringMap.empty int)).
-Definition infinite_loop_ir := (compile_program (infinite_loop) (StringMap.empty int)).
-Definition if_ir := (compile_program (trivial_if "a" "b" 0) (StringMap.empty int)).
-Definition seq_ir := (compile_program (trivial_seq "a" "b" 42) (StringMap.empty int)).
-Definition nested_if_ir := (compile_program (nested_if "a" "b" 42 43) (StringMap.empty int)).
-Definition nested_if2_ir := (compile_program (nested_if2 "a" "b" 42 43) (StringMap.empty int)).
+  Definition compile_program (s : stmt) (env : StringMap.t int) :
+    option program :=
+    '(_, _, ir) <- compile 0 s env;;
+    ret (compile_imp_cvir ir).
 
 
-(* Compute infinite_loop_ir. *)
-(* Compute seq_ir. *)
-(* Compute if_ir. *)
-(* Compute nested_if_ir. *)
-(* Compute nested_if2_ir. *)
-(* Compute fact_ir. *)
+
+  Definition fact_ir := (compile_program (fact "a" "b" 5) (StringMap.empty int)).
+  Definition infinite_loop_ir := (compile_program (infinite_loop) (StringMap.empty int)).
+  Definition if_ir := (compile_program (trivial_if "a" "b" 0) (StringMap.empty int)).
+  Definition seq_ir := (compile_program (trivial_seq "a" "b" 42) (StringMap.empty int)).
+  Definition nested_if_ir := (compile_program (nested_if "a" "b" 42 43) (StringMap.empty int)).
+  Definition nested_if2_ir := (compile_program (nested_if2 "a" "b" 42 43) (StringMap.empty int)).
+
+
+  (* Compute infinite_loop_ir. *)
+  (* Compute seq_ir. *)
+  (* Compute if_ir. *)
+  (* Compute nested_if_ir. *)
+  (* Compute nested_if2_ir. *)
+  (* Compute fact_ir. *)
+
+
 End Imp2Cvir.
